Cleaned up tree code creation just a little bit

TreeCodeConversion.thy
@@ -2,52 +2,55 @@ theory TreeCodeConversion
   imports TreeCode Closure
 begin
 
-primrec compile :: "dexpr \<Rightarrow> tree_code list" where
-  "compile (DVar x) = [TLookup x]"
-| "compile (DConst k) = [TPushCon k]"
-| "compile (DLam t e) = [TPushLam (compile e)]"
-| "compile (DApp e\<^sub>1 e\<^sub>2) = TEnter # compile e\<^sub>1 @ compile e\<^sub>2 @ [TApply]"
+primrec compile :: "dexpr \<Rightarrow> tree_code list \<Rightarrow> tree_code list" where
+  "compile (DVar x) cd = TLookup x # cd"
+| "compile (DConst k) cd = TPushCon k # cd"
+| "compile (DLam t e) cd = TPushLam (compile e []) # cd"
+| "compile (DApp e\<^sub>1 e\<^sub>2) cd = TEnter # compile e\<^sub>1 (compile e\<^sub>2 (TApply # cd))"
 
 primrec compile_closure :: "closure \<Rightarrow> tclosure" where
   "compile_closure (CConst k) = TConst k"
-| "compile_closure (CLam t cs e) = TLam (map compile_closure cs) (compile e)"
+| "compile_closure (CLam t cs e) = TLam (map compile_closure cs) (compile e [])"
 
 fun compile_stack :: "cframe list \<Rightarrow> tree_code_state" where
   "compile_stack [] = TS [] [] []"
 | "compile_stack (CApp1 cs e # s) = (case compile_stack s of 
-      TS vs envs cd \<Rightarrow> TS vs (map compile_closure cs # envs) (compile e @ TApply # cd))"
+      TS vs envs cd \<Rightarrow> TS vs (map compile_closure cs # envs) (compile e (TApply # cd)))"
 | "compile_stack (CApp2 c # s) = (case compile_stack s of 
       TS vs envs cd \<Rightarrow> TS (compile_closure c # vs) envs (TApply # cd))"
 | "compile_stack (CReturn # s) = compile_stack s"
 
 primrec compile_state :: "closure_state \<Rightarrow> tree_code_state" where
   "compile_state (CSE s cs e) = (case compile_stack s of 
-      TS vs envs cd \<Rightarrow> TS vs (map compile_closure cs # envs) (compile e @ cd))"
+      TS vs envs cd \<Rightarrow> TS vs (map compile_closure cs # envs) (compile e cd))"
 | "compile_state (CSC s c) = (case compile_stack s of 
       TS vs envs cd \<Rightarrow> TS (compile_closure c # vs) envs cd)"
 
-lemma [dest]: "TLookup x # cd = compile e @ cd' \<Longrightarrow> (e = DVar x \<Longrightarrow> cd' = cd \<Longrightarrow> P) \<Longrightarrow> P"
+lemma [simp]: "compile e cd @ cd' = compile e (cd @ cd')"
+  by (induction e arbitrary: cd) simp_all
+
+lemma [dest]: "TLookup x # cd = compile e cd' \<Longrightarrow> (e = DVar x \<Longrightarrow> cd' = cd \<Longrightarrow> P) \<Longrightarrow> P"
   by (induction e) simp_all
 
-lemma [dest]: "TPushCon k # cd = compile e @ cd' \<Longrightarrow> (e = DConst k \<Longrightarrow> cd' = cd \<Longrightarrow> P) \<Longrightarrow> P"
+lemma [dest]: "TPushCon k # cd = compile e cd' \<Longrightarrow> (e = DConst k \<Longrightarrow> cd' = cd \<Longrightarrow> P) \<Longrightarrow> P"
   by (induction e) simp_all
 
-lemma [dest]: "TPushLam cd'' # cd = compile e @ cd' \<Longrightarrow> 
-    \<exists>t e'. e = DLam t e' \<and> cd'' = compile e' \<and> cd' = cd"
+lemma [dest]: "TPushLam cd'' # cd = compile e cd' \<Longrightarrow> 
+    \<exists>t e'. e = DLam t e' \<and> cd'' = compile e' [] \<and> cd' = cd"
   by (induction e) simp_all
 
-lemma [dest]: "TEnter # cd = compile e @ cd' \<Longrightarrow> 
-    \<exists>e\<^sub>1 e\<^sub>2. e = DApp e\<^sub>1 e\<^sub>2 \<and> cd = compile e\<^sub>1 @ compile e\<^sub>2 @ TApply # cd'"
+lemma [dest]: "TEnter # cd = compile e cd' \<Longrightarrow> 
+    \<exists>e\<^sub>1 e\<^sub>2. e = DApp e\<^sub>1 e\<^sub>2 \<and> cd = compile e\<^sub>1 (compile e\<^sub>2 (TApply # cd'))"
   by (induction e) simp_all
 
-lemma [dest]: "TApply # cd = compile e @ cd' \<Longrightarrow> P"
+lemma [dest]: "TApply # cd = compile e cd' \<Longrightarrow> P"
   by (induction e) simp_all
 
 lemma [dest]: "compile_closure c = TConst k \<Longrightarrow> c = CConst k"
   by (induction c) simp_all
 
 lemma [dest]: "compile_closure c = TLam env cd \<Longrightarrow> 
-    \<exists>t cs e. c = CLam t cs e \<and> env = map compile_closure cs \<and> cd = compile e"
+    \<exists>t cs e. c = CLam t cs e \<and> env = map compile_closure cs \<and> cd = compile e []"
   by (induction c) simp_all
 
 primrec all_returnc :: "cframe list \<Rightarrow> bool" where
@@ -99,11 +102,11 @@ qed (simp_all split: tree_code_state.splits)
 lemma compile_stack_to_pushlam [simp]: "TS vs (env # envs) (TPushLam cd' # cd) = compile_stack s \<Longrightarrow> 
   \<exists>sr cs s' cd'' t e. s = sr @ CApp1 cs (DLam t e) # s' \<and> all_returnc sr \<and>  
     compile_stack s' = TS vs envs cd'' \<and> env = map compile_closure cs \<and> cd = TApply # cd'' \<and> 
-      compile e = cd'"
+      compile e [] = cd'"
 proof (induction s rule: compile_stack.induct)
   case (2 cs e s)
   then obtain s' where TS: "compile_stack s = TS vs envs s'" by (cases "compile_stack s") simp_all 
-  moreover with 2 obtain t e' where "e = DLam t e' \<and> compile e' = cd'" by auto
+  moreover with 2 obtain t e' where "e = DLam t e' \<and> compile e' [] = cd'" by auto
   moreover from 2 TS have "env = map compile_closure cs" by simp
   moreover from 2 TS have "cd = TApply # s'" by auto
   ultimately show ?case by fastforce
@@ -111,29 +114,29 @@ next
   case (4 s)
   then obtain sr cs s' cd'' t e' where "s = sr @ CApp1 cs (DLam t e') # s' \<and> all_returnc sr \<and> 
     compile_stack s' = TS vs envs cd'' \<and> env = map compile_closure cs \<and> cd = TApply # cd'' \<and> 
-      compile e' = cd'" by fastforce
+      compile e' [] = cd'" by fastforce
   hence "CReturn # s = (CReturn # sr) @ CApp1 cs (DLam t e') # s' \<and>
     all_returnc (CReturn # sr) \<and> compile_stack s' = TS vs envs cd'' \<and> 
-      env = map compile_closure cs \<and> cd = TApply # cd'' \<and> compile e' = cd'" by simp
+      env = map compile_closure cs \<and> cd = TApply # cd'' \<and> compile e' [] = cd'" by simp
   thus ?case by fastforce
 qed (simp_all split: tree_code_state.splits)
 
 lemma compile_stack_to_enter [simp]: "TS vs (env # envs) (TEnter # cd) = compile_stack s \<Longrightarrow> 
   \<exists>sr s' cd' cs e\<^sub>1 e\<^sub>2. s = sr @ CApp1 cs (DApp e\<^sub>1 e\<^sub>2) # s' \<and> all_returnc sr \<and>  
     compile_stack s' = TS vs envs cd' \<and> env = map compile_closure cs \<and> 
-      cd = compile e\<^sub>1 @ compile e\<^sub>2 @ TApply # TApply # cd'" 
+      cd = compile e\<^sub>1 (compile e\<^sub>2 (TApply # TApply # cd'))" 
 proof (induction s rule: compile_stack.induct)
   case (2 cs e s)
   then obtain cd' where TS: "compile_stack s = TS vs envs cd' \<and> env = map compile_closure cs \<and> 
-    TEnter # cd = compile e @ TApply # cd'" by (cases "compile_stack s") simp_all
+    TEnter # cd = compile e (TApply # cd')" by (cases "compile_stack s") simp_all
   moreover then obtain e\<^sub>1 e\<^sub>2 where "e = DApp e\<^sub>1 e\<^sub>2 \<and> 
-    cd = compile e\<^sub>1 @ compile e\<^sub>2 @ TApply # TApply # cd'" by fastforce
+    cd = compile e\<^sub>1 (compile e\<^sub>2 (TApply # TApply # cd'))" by fastforce
   ultimately show ?case by fastforce
 next
   case (4 s)
   from 4 obtain sr s' cd' cs e\<^sub>1 e\<^sub>2 where "s = sr @ CApp1 cs (DApp e\<^sub>1 e\<^sub>2) # s' \<and> all_returnc sr \<and>
     compile_stack s' = TS vs envs cd' \<and> env = map compile_closure cs \<and> 
-      cd = compile e\<^sub>1 @ compile e\<^sub>2 @ TApply # TApply # cd'" by fastforce
+      cd = compile e\<^sub>1 (compile e\<^sub>2 (TApply # TApply # cd'))" by fastforce
   moreover hence "CReturn # s = (CReturn # sr) @ CApp1 cs (DApp e\<^sub>1 e\<^sub>2) # s' \<and> 
     all_returnc (CReturn # sr)" by simp
   ultimately show ?case by fastforce
@@ -181,10 +184,10 @@ proof (induction \<Sigma>)
 qed (auto split: tree_code_state.splits)
 
 lemma compile_to_pushlam [simp]: "TS vs (env # envs) (TPushLam cd' # cd) = compile_state \<Sigma> \<Longrightarrow> 
-  (\<exists>s cs t e. compile_stack s = TS vs envs cd \<and> env = map compile_closure cs \<and> cd' = compile e \<and> 
+  (\<exists>s cs t e. compile_stack s = TS vs envs cd \<and> env = map compile_closure cs \<and> cd' = compile e [] \<and> 
     \<Sigma> = CSE s cs (DLam t e)) \<or> (\<exists>sr s vs' c cd'' cs t e. compile_stack s = TS vs' envs cd'' \<and> 
       cd = TApply # cd'' \<and> vs = compile_closure c # vs' \<and> env = map compile_closure cs \<and> 
-        all_returnc sr \<and> cd' = compile e \<and> \<Sigma> = CSC (sr @ CApp1 cs (DLam t e) # s) c)"
+        cd' = compile e [] \<and> all_returnc sr \<and> \<Sigma> = CSC (sr @ CApp1 cs (DLam t e) # s) c)"
 proof (induction \<Sigma>)
   case (CSC s c)
   then obtain vs' where "TS vs' (env # envs) (TPushLam cd' # cd) = compile_stack s \<and> 
@@ -194,10 +197,10 @@ qed (auto split: tree_code_state.splits)
 
 lemma compile_to_enter [simp]: "TS vs (env # envs) (TEnter # cd) = compile_state \<Sigma> \<Longrightarrow> 
   (\<exists>s cs e\<^sub>1 e\<^sub>2 cd'. \<Sigma> = CSE s cs (DApp e\<^sub>1 e\<^sub>2) \<and> compile_stack s = TS vs envs cd' \<and> 
-    env = map compile_closure cs \<and> cd = compile e\<^sub>1 @ compile e\<^sub>2 @ TApply # cd') \<or>
+    env = map compile_closure cs \<and> cd = compile e\<^sub>1 (compile e\<^sub>2 (TApply # cd'))) \<or>
       (\<exists>sr s c vs' cd' cs e\<^sub>1 e\<^sub>2. \<Sigma> = CSC (sr @ CApp1 cs (DApp e\<^sub>1 e\<^sub>2) # s) c \<and> 
         vs = compile_closure c # vs' \<and> compile_stack s = TS vs' envs cd' \<and> all_returnc sr \<and>
-          env = map compile_closure cs \<and> cd = compile e\<^sub>1 @ compile e\<^sub>2 @ TApply # TApply # cd')" 
+          env = map compile_closure cs \<and> cd = compile e\<^sub>1 (compile e\<^sub>2 (TApply # TApply # cd')))" 
 proof (induction \<Sigma>) 
   case (CSC s c)
   then obtain vs' where "vs = compile_closure c # vs' \<and> 
@@ -284,7 +287,7 @@ next
   thus ?case
   proof (induction \<Sigma>\<^sub>c)
     case (CSE s cs e')
-    then obtain t e where S: "env = map compile_closure cs \<and> cd' = compile e \<and> 
+    then obtain t e where S: "env = map compile_closure cs \<and> cd' = compile e [] \<and> 
       compile_stack s = TS vs envs cd \<and> CSE s cs e' = CSE s cs (DLam t e)" 
         using compile_to_pushlam by blast
     have "CSE s cs (DLam t e) \<leadsto>\<^sub>c CSC s (CLam t cs e)" by simp
@@ -294,7 +297,7 @@ next
     case (CSC s c)
     then obtain rs s' vs' cd'' cs t e where E: "compile_stack s' = TS vs' envs cd'' \<and> 
       cd = TApply # cd'' \<and> vs = compile_closure c # vs' \<and> env = map compile_closure cs \<and> 
-        cd' = compile e \<and> s = rs @ CApp1 cs (DLam t e) # s' \<and> all_returnc rs" 
+        cd' = compile e [] \<and> s = rs @ CApp1 cs (DLam t e) # s' \<and> all_returnc rs" 
           using compile_to_pushlam by blast
     have "CSE (CApp2 c # s') cs (DLam t e) \<leadsto>\<^sub>c CSC (CApp2 c # s') (CLam t cs e)" by simp
     moreover have "CSC (CApp1 cs (DLam t e) # s') c \<leadsto>\<^sub>c CSE (CApp2 c # s') cs (DLam t e)" by simp
@@ -311,7 +314,7 @@ next
   proof (induction \<Sigma>\<^sub>c)
     case (CSE s cs e)
     then obtain e\<^sub>1 e\<^sub>2 cd' where E: "e = DApp e\<^sub>1 e\<^sub>2 \<and> compile_stack s = TS vs envs cd' \<and> 
-      env = map compile_closure cs \<and> cd = compile e\<^sub>1 @ compile e\<^sub>2 @ TApply # cd'" 
+      env = map compile_closure cs \<and> cd = compile e\<^sub>1 (compile e\<^sub>2 (TApply # cd'))" 
         using compile_to_enter by blast
     have "CSE s cs (DApp e\<^sub>1 e\<^sub>2) \<leadsto>\<^sub>c CSE (CApp1 cs e\<^sub>2 # s) cs e\<^sub>1" by simp
     hence "iter (\<leadsto>\<^sub>c) (CSE s cs (DApp e\<^sub>1 e\<^sub>2)) (CSE (CApp1 cs e\<^sub>2 # s) cs e\<^sub>1)" 
@@ -321,7 +324,7 @@ next
     case (CSC s c)
     then obtain rs s' vs' cd' cs e\<^sub>1 e\<^sub>2 where S: "s = rs @ CApp1 cs (DApp e\<^sub>1 e\<^sub>2) # s' \<and> 
       vs = compile_closure c # vs' \<and> compile_stack s' = TS vs' envs cd' \<and> all_returnc rs \<and> 
-        env = map compile_closure cs \<and> cd = compile e\<^sub>1 @ compile e\<^sub>2 @ TApply # TApply # cd'" 
+        env = map compile_closure cs \<and> cd = compile e\<^sub>1 (compile e\<^sub>2 (TApply # TApply # cd'))" 
       using compile_to_enter by blast
     have "CSC (CApp1 cs (DApp e\<^sub>1 e\<^sub>2) # s') c \<leadsto>\<^sub>c CSE (CApp2 c # s') cs (DApp e\<^sub>1 e\<^sub>2)" by simp
     moreover have "CSE (CApp2 c # s') cs (DApp e\<^sub>1 e\<^sub>2) \<leadsto>\<^sub>c CSE (CApp1 cs e\<^sub>2 # CApp2 c # s') cs e\<^sub>1" 
@@ -337,7 +340,7 @@ next
   then obtain rs s c c' where S: "\<Sigma>\<^sub>c = CSC (rs @ CApp2 c' # s) c \<and> v = compile_closure c \<and> 
     compile_closure c' = TLam env cd' \<and> compile_stack s = TS vs envs cd \<and> all_returnc rs" 
       using compile_to_apply by fastforce
-  then obtain t cs e where C: "c' = CLam t cs e \<and> env = map compile_closure cs \<and> cd' = compile e" 
+  then obtain t cs e where C: "c' = CLam t cs e \<and> env = map compile_closure cs \<and> cd' = compile e []" 
     by fastforce
   have "CSC (CApp2 (CLam t cs e) # s) c \<leadsto>\<^sub>c CSE (CReturn # s) (c # cs) e" by simp
   moreover from S have "iter (\<leadsto>\<^sub>c) (CSC (rs @ CApp2 (CLam t cs e) # s) c) 
@@ -370,22 +373,23 @@ next
   case (evc_lam s cs t e)
   obtain vs envs cd where S: "compile_stack s = TS vs envs cd" 
     by (induction s rule: compile_stack.induct) (simp_all split: tree_code_state.splits)
-  have "TS vs (map compile_closure cs # envs) (TPushLam (compile e) # cd) \<leadsto>\<^sub>t 
-    TS (TLam (map compile_closure cs) (compile e) # vs) envs cd" by simp
-  hence "iter (\<leadsto>\<^sub>t) (TS vs (map compile_closure cs # envs) (TPushLam (compile e) # cd)) 
-      (TS (TLam (map compile_closure cs) (compile e) # vs) envs cd)" by (metis iter_step iter_refl)
+  have "TS vs (map compile_closure cs # envs) (TPushLam (compile e []) # cd) \<leadsto>\<^sub>t 
+    TS (TLam (map compile_closure cs) (compile e []) # vs) envs cd" by simp
+  hence "iter (\<leadsto>\<^sub>t) (TS vs (map compile_closure cs # envs) (TPushLam (compile e []) # cd)) 
+    (TS (TLam (map compile_closure cs) (compile e []) # vs) envs cd)" 
+      by (metis iter_step iter_refl)
   with S show ?case by simp
 next
   case (evc_app s cs e\<^sub>1 e\<^sub>2)
   obtain vs envs cd where S: "compile_stack s = TS vs envs cd" 
     by (induction s rule: compile_stack.induct) (simp_all split: tree_code_state.splits)
-  have "TS vs (map compile_closure cs # envs) (TEnter # compile e\<^sub>1 @ compile e\<^sub>2 @ TApply # cd) \<leadsto>\<^sub>t
+  have "TS vs (map compile_closure cs # envs) (TEnter # compile e\<^sub>1 (compile e\<^sub>2 (TApply # cd))) \<leadsto>\<^sub>t
       TS vs (map compile_closure cs # map compile_closure cs # envs) 
-        (compile e\<^sub>1 @ compile e\<^sub>2 @ TApply # cd)" by simp
+        (compile e\<^sub>1 (compile e\<^sub>2 (TApply # cd)))" by simp
   hence "iter (\<leadsto>\<^sub>t) (TS vs (map compile_closure cs # envs) 
-    (TEnter # compile e\<^sub>1 @ compile e\<^sub>2 @ TApply # cd))
+    (TEnter # compile e\<^sub>1 (compile e\<^sub>2 (TApply # cd))))
       (TS vs (map compile_closure cs # map compile_closure cs # envs) 
-        (compile e\<^sub>1 @ compile e\<^sub>2 @ TApply # cd))" by (metis iter_step iter_refl)
+        (compile e\<^sub>1 (compile e\<^sub>2 (TApply # cd))))" by (metis iter_step iter_refl)
   with S show ?case by simp
 next
   case (retc_app1 cs e\<^sub>2 s c\<^sub>1)
@@ -396,12 +400,13 @@ next
   case (retc_app2 t cs e\<^sub>1 s c\<^sub>2)
   obtain vs envs cd where S: "compile_stack s = TS vs envs cd" 
     by (induction s rule: compile_stack.induct) (simp_all split: tree_code_state.splits)
-  have "TS (compile_closure c\<^sub>2 # TLam (map compile_closure cs) (compile e\<^sub>1) # vs) envs (TApply # cd) 
-    \<leadsto>\<^sub>t TS vs ((compile_closure c\<^sub>2 # map compile_closure cs) # envs) ((compile e\<^sub>1) @ cd)" 
-      by (metis evt_apply)
-  hence "iter (\<leadsto>\<^sub>t) (TS (compile_closure c\<^sub>2 # TLam (map compile_closure cs) (compile e\<^sub>1) # vs) envs 
-    (TApply # cd))
-      (TS vs ((compile_closure c\<^sub>2 # map compile_closure cs) # envs) (compile e\<^sub>1 @ cd))" 
+  have "TS (compile_closure c\<^sub>2 # TLam (map compile_closure cs) (compile e\<^sub>1 []) # vs) 
+    envs (TApply # cd) \<leadsto>\<^sub>t 
+      TS vs ((compile_closure c\<^sub>2 # map compile_closure cs) # envs) (compile e\<^sub>1 [] @ cd)" 
+        by (metis evt_apply)
+  hence "iter (\<leadsto>\<^sub>t) (TS (compile_closure c\<^sub>2 # TLam (map compile_closure cs) (compile e\<^sub>1 []) # vs) 
+    envs (TApply # cd))
+      (TS vs ((compile_closure c\<^sub>2 # map compile_closure cs) # envs) (compile e\<^sub>1 [] @ cd))" 
     by (metis iter_step iter_refl)
   with S show ?case by simp
 qed simp_all
