Compiler.thy
@@ -2,7 +2,7 @@ theory Compiler
   imports AlgorithmicTypechecking Printing StackConversion
 begin
 
-theorem tc_terminationn: "typechecks e \<Longrightarrow> flatten_code (compile (convert e)) = cd \<Longrightarrow> 
+theorem tc_terminationn: "typechecks e \<Longrightarrow> flatten_code (compile (convert e) []) = cd \<Longrightarrow> 
   \<exists>v. valn v \<and> iter (\<leadsto>\<^sub>n) e v \<and> 
     (\<exists>h v\<^sub>h. iter (\<leadsto>\<^sub>h) (HS hempty [] [[]] [length cd] cd) (HS h [v\<^sub>h] [] [] cd) \<and> 
       print_hclosure h v\<^sub>h = print_nexpr v)"
@@ -20,10 +20,11 @@ proof -
   with VN have VC: "print_closure c = print_nexpr v\<^sub>n" by simp
   from EC have "iter (\<leadsto>\<^sub>t) (compile_state (CSE [] [] (convert e))) (compile_state (CSC [] c))" 
     by (metis iter_completet)
-  hence ET: "iter (\<leadsto>\<^sub>t) (TS [] [[]] (compile (convert e))) (TS [compile_closure c] [] [])" by simp
-  assume C: "flatten_code (compile (convert e)) = cd"
-  hence "unflatten_code cd (length cd) = compile (convert e)" by auto
-  hence UB: "unflatten_state (BS [] [[]] [length cd] cd) = TS [] [[]] (compile (convert e))" 
+  hence ET: "iter (\<leadsto>\<^sub>t) (TS [] [[]] (compile (convert e) [])) (TS [compile_closure c] [] [])" 
+    by simp
+  assume C: "flatten_code (compile (convert e) []) = cd"
+  hence "unflatten_code cd (length cd) = compile (convert e) []" by auto
+  hence UB: "unflatten_state (BS [] [[]] [length cd] cd) = TS [] [[]] (compile (convert e) [])" 
     by simp
   from C have "orderly_state (BS [] [[]] [length cd] cd)" by auto
   with ET UB obtain v\<^sub>b where EB: 
